\begin{solution}
    因为$nT(n)=(n-2)T(n-1)+2$\\
    所以$nT(n)=(n-1)T(n-1)+2-T(n-1)$\\
    两边分别以1为步长自n向下求和：
    \begin{displaymath}
        \sum_{i = n - \lceil n - 1 \rceil +1}^{n} iT(i) = 
        \sum_{j = n - \lceil n - 1 \rceil}^{n - 1} jT(j) + 2 - T(j) 
    \end{displaymath}
    左右消项：
    \begin{displaymath}
        nT(n) = (n - \lceil n - 1 \rceil)T(n - \lceil n - 1 \rceil) + 2 \lceil n - 1 \rceil - \sum_{i = n - \lceil n - 1 \rceil}^{n - 1} T(i)
    \end{displaymath}
    由于$n - \lceil n - 1 \rceil \le 1$且$\forall x, T(x)>=0$故：
    \begin{displaymath}
        (n - \lceil n - 1 \rceil)T(n - \lceil n - 1 \rceil) - \sum_{i = n - \lceil n - 1 \rceil}^{n - 1} T(i) \le 0
    \end{displaymath}   
    于是：
    $$T(n)\le \frac{2\lceil n - 1 \rceil}{n} \le 2$$
    又由$nT(n)=(n-2)T(n-1)+2$可知：
    \begin{align*}
        T(n)=\frac{n-2}{n}T(n-1)+\frac{2}{n}
    \end{align*}
    又已知$\forall n>0,T(n) \le 2$成立，所以$\forall 1 < n \le 2$有：
    \begin{align*}
        T(n) \le& ~2 \cdot\frac{n-2}{n}+ \frac{2}{n}\\
             =& ~2 - \frac{2}{n}\\
             \le& ~1
    \end{align*}
    下面证明：若$T(k)\le 1$，则$T(k+1) \le 1$.\\
    \begin{align*}
        T(n) =& ~\frac{n-2}{n}T(n-1)+\frac{2}{n}\\
        \le& ~\frac{n-2}{n}+\frac{2}{n}\\
        =& ~1
    \end{align*}
    于是归纳得到：$\forall n>1,T(n)\le 1$.\\
    综合$T(n)$的约束：
    \begin{align*}
       T(n) \le \left\{
        \begin{aligned}
            2& \quad 0 < n \le 1 \\
            1& \quad n > 1
        \end{aligned}
       \right.
    \end{align*}
    根据已知$nT(n)$的式子可继续推导：
    \begin{align*}
        nT(n) =&~ (n - \lceil n - 1 \rceil)T(n - \lceil n - 1 \rceil) + 2 \lceil n - 1 \rceil - \sum_{i = n - \lceil n - 1 \rceil}^{n - 1} T(i)\\
        \ge&~ 2 \lceil n - 1 \rceil - \sum_{i = n - \lceil n - 1 \rceil}^{n - 1} T(i)\\
    \end{align*}
    由$T(n)$的约束，知以下两式：
    $$T(n-\lceil n - 1 \rceil) \le 2$$
    $$\forall k \ge n-\lceil n - 1 \rceil+1, T(k) \le 1$$
    进而：
    \begin{align*}
        nT(n) \ge&~ 2 \lceil n - 1 \rceil - \sum_{i = n - \lceil n - 1 \rceil}^{n - 1} T(i)\\
        \ge&~ 2 \lceil n - 1 \rceil - 2 - 1 \cdot (\lceil n - 1 \rceil - 1)\\
        =&~ \lceil n - 1 \rceil - 1
    \end{align*}
    因此：
    \begin{align*}
        T(n) \ge&~ \frac{\lceil n - 1 \rceil - 1}{n}\\
        \ge&~ \frac{n - 2}{n}\\
        =&~ 1-\frac{2}{n}
    \end{align*}
    即可知：$\forall n \ge 3,T(n) \ge \frac{1}{3}$\\
    综上所述，$\forall n \ge 3, \frac{1}{3} \le T(n) \le 1$，即$T(n)=\Theta(1)$
\end{solution}